working/composition/event_based_refinement/load_balancer/service_correspondence/shared/AbstractServiceSM.t.dfy
@@ -12,20 +12,10 @@ abstract module AbstractServiceSM {
     ghost predicate Init(c: Constants, v: Variables)
     ghost predicate Next(c: Constants, v: Variables, v': Variables, msgOps: MessageOps)
 
-    ghost function MarshallServiceRequest(request: ServiceRequest): seq<byte>
-    ghost function MarshallServiceReply(reply: ServiceReply): seq<byte>
     ghost function ParseServiceRequest(bytes: seq<byte>): Option<ServiceRequest>
     ghost function ParseServiceReply(bytes: seq<byte>): Option<ServiceReply>
-    
-    lemma MarshallParseInverse(bytes: seq<byte>)
-        ensures ParseServiceRequest(bytes).Some? ==> MarshallServiceRequest(ParseServiceRequest(bytes).value) == bytes
-        ensures ParseServiceReply(bytes).Some? ==> MarshallServiceReply(ParseServiceReply(bytes).value) == bytes
-        ensures forall req :: bytes == MarshallServiceRequest(req) ==> ParseServiceRequest(bytes).Some?
-        ensures forall repl :: bytes == MarshallServiceReply(repl) ==> ParseServiceReply(bytes).Some?
 
-    lemma ParseMarshallServiceRequestInverse(req: ServiceRequest)
-        ensures ParseServiceRequest(MarshallServiceRequest(req)).Some? && ParseServiceRequest(MarshallServiceRequest(req)).value == req
-
-    lemma ParseMarshallServiceReplyInverse(repl: ServiceReply)
-        ensures ParseServiceReply(MarshallServiceReply(repl)).Some? && ParseServiceReply(MarshallServiceReply(repl)).value == repl
+    lemma ParseOneToOne(m1: seq<byte>, m2: seq<byte>)
+        ensures ParseServiceRequest(m1).Some? && ParseServiceRequest(m2).Some? && ParseServiceRequest(m1).value == ParseServiceRequest(m2).value ==> m1 == m2
+        ensures ParseServiceReply(m1).Some? && ParseServiceReply(m2).Some? && ParseServiceReply(m1).value == ParseServiceReply(m2).value ==> m1 == m2
 }
